src/lambda_verus/typing/ghost.v
@@ -5,7 +5,7 @@ From lrust.typing Require Import own.
 Set Default Proof Using "Type".
 
 Section ghost.
-  Context `{!typeG Σ}.
+  Context `{!typeG Σ, !cnaInv_logicG Σ}.
 
   Program Definition ghost_ty {𝔄} (ty: type 𝔄) : type (ghostₛ 𝔄) := @ty_of_st _ _ (ghostₛ 𝔄)
     ({|
@@ -19,7 +19,7 @@ Section ghost.
   Next Obligation. move=> *. trivial. Qed.
   Next Obligation. move=> *. trivial. Qed.
   Next Obligation. intros. iIntros. done. Qed.
-  Next Obligation. intros 𝔄 ty κ x n d g tid ξ R Hin. exfalso. simpl in Hin. set_solver. Qed.
+  (* [st_guard_proph] obligation elided: prophecy stripped. *)
   Next Obligation. done. Qed.
   
   Global Instance tracked_ne {𝔄} : NonExpansive (@ghost_ty 𝔄).
@@ -27,9 +27,8 @@ Section ghost.
 
   Global Instance ghost_send {𝔄} (ty : type 𝔄) : Send (ghost_ty ty).
   Proof.
-    intros. split; trivial. iIntros. iApply step_fupdN_intro; first done. iNext.
-    iExists x, 0%nat. iModIntro. iFrame. simpl.
-    replace (d0 + 0)%nat with d0 by lia. iFrame "#". done.
+    (* [send_change_tid] field elided: concurrency stripped. *)
+    intros. split; trivial.
   Qed.
   
   Global Instance ghost_sync {𝔄} (ty : type 𝔄) : Sync (ghost_ty ty).
@@ -38,23 +37,22 @@ Section ghost.
   Global Instance ghost_copy {𝔄} (ty : type 𝔄) : Copy (ghost_ty ty).
   Proof. split; try done. typeclasses eauto. Qed.
 
-  Lemma ghost_resolve {𝔄} (ty: type 𝔄) E L : resolve E L (ghost_ty ty) (const (const True)).
-  Proof. apply resolve_just. Qed.
+  (* [ghost_resolve] removed along with [resolve]. *)
   
   Lemma ghost_constant {𝔄} E L I (ty : type 𝔄) (c: ~~𝔄) :
     typed_instr E L I
       +[] (new [ #0 ]%E)
       (λ q, +[q ◁ own_ptr 0 (ghost_ty ty)])
-      (λ post '-[], λ mask π, ∀ l, post -[(l, c)] mask π).
+      (λ post '-[], λ mask, ∀ l, post -[(l, c)] mask).
   Proof.
-    move => tid postπ mask iκs [].
-    iIntros "LFT TIME #PROPH UNIQ E L $ TY #Obs" => /=.
+    move => tid post mask iκs [].
+    iIntros "LFT #TIME #UNIQ E L $ TY %Obs" => /=.
     iMod (persistent_time_receipt_0) as "⧖".
-    iApply (wp_persistent_time_receipt with "TIME ⧖"); [done|]. iIntros "_ ⧖".
+    iApply (wp_persistent_time_receipt _ with "TIME ⧖"); [done|solve_ndisj|]. iIntros "_ ⧖".
     iApply wp_new=>//. iIntros "!>" (l) "(† & ↦)". iExists -[(l, c)]. iFrame. iSplitL.
     - iExists (#l). iSplit; first done. iSplit; last done.
       unfold own_ptr, ty_gho. rewrite !freeable_util.freeable_sz_full. iFrame. done.
-    - iApply (proph_obs_impl with "Obs"). done.
+    - iPureIntro. apply Obs.
   Qed.
   
   Lemma ghost_snapshot {𝔄} E L I p (ty : type 𝔄) :
@@ -62,17 +60,17 @@ Section ghost.
       +[p ◁ ty]
       (new [ #0 ]%E)
       (λ q, +[p ◁ ty; q ◁ own_ptr 0 (ghost_ty ty)])
-      (λ post '-[x], λ mask π, ∀ l, post -[x; (l, x)] mask π).
+      (λ post '-[x], λ mask, ∀ l, post -[x; (l, x)] mask).
   Proof.
-    move => tid postπ mask iκs [x []].
-    iIntros "LFT TIME #PROPH UNIQ E L $ [T TY] #Obs" => /=.
+    move => tid post mask iκs [x []].
+    iIntros "LFT #TIME #UNIQ E L $ [T TY] %Obs" => /=.
     iMod (persistent_time_receipt_0) as "⧖".
-    iApply (wp_persistent_time_receipt with "TIME ⧖"); [done|]. iIntros "_ ⧖".
+    iApply (wp_persistent_time_receipt _ with "TIME ⧖"); [done|solve_ndisj|]. iIntros "_ ⧖".
     iApply wp_new=>//. iIntros "!>" (l) "(† & ↦)". iExists -[x; (l, x)]. iFrame "T".
     iFrame. iSplitL.
     - iExists (#l). iSplit; first done. iSplit; last done.
       unfold own_ptr, ty_gho. rewrite !freeable_util.freeable_sz_full. iFrame. done.
-    - iApply (proph_obs_impl with "Obs"). done.
+    - iPureIntro. apply Obs.
   Qed.
   
   Lemma ghost_compute {𝔄 𝔅 ℭ} E L I p1 p2 (ty1 : type 𝔄) (ty2 : type 𝔅) (ty: type ℭ)
@@ -81,18 +79,17 @@ Section ghost.
       +[p1 ◁ ty1; p2 ◁ ty2]
       (new [ #0 ]%E)
       (λ q, +[p1 ◁ ty1; p2 ◁ ty2; q ◁ own_ptr 0 (ghost_ty ty)])
-      (λ post '-[x; y], λ mask π, ∀ l, post -[x; y; (l, f x y)] mask π).
+      (λ post '-[x; y], λ mask, ∀ l, post -[x; y; (l, f x y)] mask).
   Proof.
-    move => tid postπ mask iκs [x [y []]].
-    iIntros "LFT TIME #PROPH UNIQ E L $ [T1 [T2 TY]] #Obs" => /=.
+    move => tid post mask iκs [x [y []]].
+    iIntros "LFT #TIME #UNIQ E L $ [T1 [T2 TY]] %Obs" => /=.
     iMod (persistent_time_receipt_0) as "⧖".
-    iApply (wp_persistent_time_receipt with "TIME ⧖"); [done|]. iIntros "_ ⧖".
+    iApply (wp_persistent_time_receipt _ with "TIME ⧖"); [done|solve_ndisj|]. iIntros "_ ⧖".
     iApply wp_new=>//. iIntros "!>" (l) "(† & ↦)". iExists -[x; y; (l, f x y)].
     iFrame "T1 T2". iFrame. iSplitL.
     - iExists (#l). iSplit; first done. iSplit; last done.
       unfold own_ptr, ty_gho. rewrite !freeable_util.freeable_sz_full. iFrame. done.
-    - iApply (proph_obs_impl with "Obs"). done.
+    - iPureIntro. apply Obs.
   Qed.
 End ghost.
 
-Global Hint Resolve ghost_resolve : lrust_typing.
