src/lambda_verus/typing/local_inv.v
@@ -9,7 +9,7 @@ Set Default Proof Using "Type".
 Implicit Type 𝔄 𝔅: syn_type.
 
 Section na_dg_agree_util.
-  Context `{!typeG Σ}. 
+  Context `{!typeG Σ, !cnaInv_logicG Σ}. 
   
   Local Definition dg_tok γ (k: nat) : iProp Σ :=
       own γ (to_frac_agree (A:=leibnizO (nat)) (1/2)%Qp k).
@@ -42,7 +42,7 @@ Section na_dg_agree_util.
 End na_dg_agree_util.
 
 Section local_invariants.
-  Context `{!typeG Σ}. 
+  Context `{!typeG Σ, !cnaInv_logicG Σ}. 
 
   (*
   In Verus, the AtomicInvariant is parameterized as:
@@ -100,7 +100,7 @@ Section local_invariants.
     iIntros "[A [[%B1 B1'] C]]". iFrame. done.
   Qed.
   Next Obligation. iIntros. done. Qed.
-  Next Obligation. set_solver. Qed.
+  (* [ty_guard_proph] obligation elided: prophecy stripped. *)
   Next Obligation. iIntros. done. Qed.
   
   Program Definition local_closer_ty {𝔄 ℭ} (κ: lft) (ty: type 𝔄) (pred: (abstracted_syn_type 𝔄) → ~~ℭ → Prop) : type (local_invₛ ℭ) := ({|
@@ -124,55 +124,14 @@ Section local_invariants.
   Next Obligation. done. Qed. 
   Next Obligation. iIntros. iFrame. iIntros. done. Qed.
   Next Obligation. iIntros. done. Qed.
-  Next Obligation. set_solver. Qed.
+  (* [ty_guard_proph] obligation elided: prophecy stripped. *)
   Next Obligation. iIntros. done. Qed.
   
-  Lemma local_inv_ty_send {𝔄 ℭ} (ty: type 𝔄) (pred: (abstracted_syn_type 𝔄) → ~~ℭ → Prop)
-      : Send ty → Send (local_inv_ty ty pred).
-  Proof.
-    intros Hsend. split; [done|]. intros tid tid' x d g G H κs d0 Hineq TG TH.
-    destruct x as [[N [[γ γt] d1]] c].
-    iIntros "LFT UNIQ #TIME #Hg H #Gg G [Active [[%Hineqs DgTok] #Inv]] ⧖o".
-    iApply fupd_step_fupdN_front.
-    leaf_open "Hg" with "H" as "[cna_lifetimes back]"; first solve_ndisj.
-    iMod (cna_destroy with "Inv cna_lifetimes Active Gg G") as "[cna_lifetimes [G P]]";
-        first by solve_ndisj.
-    iMod ("back" with "cna_lifetimes") as "H". iModIntro. destruct d as [|d]; first lia.
-    simpl. iModIntro. iNext. iModIntro.
-    iDestruct "P" as (x' d' g' d00) "[DgTok1 [⧖1 [⧗ [£ [gho %Hpred]]]]]".
-    iDestruct (dg_tok_agree with "DgTok DgTok1") as "%Heqs". subst d00.
-    iCombine "⧖o ⧖1" as "⧖max".
-    iDestruct (send_change_tid tid tid' _ _ _ G H κs _ _ TG TH with "LFT UNIQ TIME Hg H Gg G gho ⧖max") as "X". Unshelve. 2: { lia. }
-    iDestruct (step_fupdN_nmono _ ((d' - d1) + d) with "X") as "X"; first lia.
-    rewrite step_fupdN_add.
-    iApply fupd_step_fupdN_front.
-    iMod (lc_step_fupdN_elim_later with "£ X") as "X". iModIntro.
-    iApply (step_fupdN_wand with "X"). iIntros "X". iMod "X".
-    iDestruct "X" as (x'' off) "[gho [⧖off [%Habs [G H]]]]".
-    iMod (dg_tok_update _ _ _ (d1+off+(d'-d1)) with "DgTok DgTok1") as "[DgTok DgTok1]".
-    iMod (cumulative_persistent_time_receipt with "TIME ⧗ ⧖off") as "#⧖offoff"; first by solve_ndisj.
-    (* very convenient we can allocate without the thread pool token *)
-    iMod (lc_zero) as "£0".
-    iMod (cumulative_time_receipt_0) as "⧗0".
-    iMod (cna_alloc tid' N with "[DgTok gho ⧗0 £0]") as (γ') "[inv active]"; last first.
-     - iModIntro. iExists (N, (γ', γt, d1+off+(d'-d1)), c), (off+(d'-d1)). iFrame "active DgTok1".
-       iSplit.
-        + iSplit. { iPureIntro. lia. } iApply "inv".
-        + iSplit. { iApply (persistent_time_receipt_mono with "⧖offoff"). lia. }
-          iFrame "G H". iPureIntro. done.
-     - iFrame.
-        iSplit. { iApply (persistent_time_receipt_mono with "⧖offoff"); lia. }
-        iSplitL "⧗0". { iApply (cumulative_time_receipt_mono with "⧗0"). lia. }
-        iSplitL "£0". { iApply (lc_weaken with "£0"). lia. }
-        rewrite Habs. done.
-  Qed.
-  
-  (* no Sync lemma *)
-  
-  Lemma local_inv_ty_resolve E L {𝔄 ℭ} (ty: type 𝔄) (pred: (abstracted_syn_type 𝔄) → ~~ℭ → Prop)
-      : resolve E L (local_inv_ty ty pred) (const (const True)).
-  Proof. apply resolve_just. Qed.
-  
+  (** [local_inv_ty_send] removed: [Send]'s [send_change_tid] field
+      is elided (concurrency is not modelled). *)
+
+  (* [local_inv_ty_resolve] removed along with [resolve]. *)
+
   Lemma typed_local_inv_alloc {𝔄 ℭ} (p1 p2 : path) (ty : type 𝔄) (pred: (abstracted_syn_type 𝔄) → ~~ℭ → Prop) (tyCN : type (ℭ * namespaceₛ)) E L I :
     typed_inv_instr E L I
       +[p1 ◁ own_ptr 0 (ghost_ty tyCN);
@@ -180,23 +139,23 @@ Section local_invariants.
        ]
       (Seq Skip Skip) I
       (const +[p2 ◁ own_ptr 0 (local_inv_ty ty pred)])
-      (λ post '-[(_, (c, N)); (_, v)], λ mask π, pred (syn_abstract v) c ∧ ∀ l γ, post -[(l, (N, γ, c))] mask π).
+      (λ post '-[(_, (c, N)); (_, v)], λ mask, pred (syn_abstract v) c ∧ ∀ l γ, post -[(l, (N, γ, c))] mask).
   Proof.
     apply typed_instr_of_skip_own2_own. { trivial. } { trivial. }
     intros l1 l2 x1 x2 d tid post mask iκs.
-    iIntros "#LFT #TIME #PROPH #UNIQ #E L I1 Gho Tra #Obs #⧖ £".
-    iMod (proph_obs_sat with "PROPH Obs") as "%Sat". { set_solver. }
+    iIntros "#LFT #TIME #UNIQ #E L I1 Gho Tra %Obs #⧖ £".
     destruct x1 as [c ns].
+    destruct Obs as [Sat Obs].
     iMod (dg_tok_alloc d) as (γt) "[tok1 tok2]".
     iMod (cumulative_time_receipt_0) as "⧗0".
     iMod (lc_zero) as "£0".
     iMod (cna_alloc tid ns with "[Tra tok1 ⧗0 £0]") as (γ) "[inv active]"; last first.
      - iModIntro. iExists (ns, (γ, γt, d), c). iFrame. iSplit; first by (iPureIntro; lia).
-       iApply (proph_obs_impl with "Obs"). intuition.
+       iPureIntro. apply Obs.
      - iNext. iExists x2, d, (S d). iFrame.
        iSplit. { iApply (persistent_time_receipt_mono with "⧖"). lia. }
        replace (d - d) with 0 by lia. iFrame.
-       iPureIntro. destruct Sat as [π1 [H1 H2]]. trivial.
+       iPureIntro. exact Sat.
   Qed.
   
   Lemma typed_local_inv_destroy {𝔄 ℭ} (p : path) (ty : type 𝔄) (pred: (abstracted_syn_type 𝔄) → ~~ℭ → Prop) E L I :
@@ -205,11 +164,11 @@ Section local_invariants.
       +[p ◁ own_ptr 0 (local_inv_ty ty pred)]
       (Seq Skip Skip)
       (const +[p ◁ own_ptr 0 (tracked_ty ty)])
-      (λ post '-[(_, (N, γ, c))], λ mask π, ∀ l v, pred (syn_abstract v) c → post -[(l, v)] mask π).
+      (λ post '-[(_, (N, γ, c))], λ mask, ∀ l v, pred (syn_abstract v) c → post -[(l, v)] mask).
   Proof.
     intros Halive. apply typed_instr_of_skip_own_own_t. { trivial. } { trivial. }
     intros l [[ns [[γ γt] d0]] c] d tid iκs post mask.
-    iIntros "#LFT #TIME #PROPH #UNIQ #E L I (active & [%Hineq tok] & #inv) #Obs #⧖ ⧗".
+    iIntros "#LFT #TIME #UNIQ #E L I (active & [%Hineq tok] & #inv) %Obs #⧖ ⧗".
     destruct I as [Il ϝ'].
     (*iAssert (∀ κ : lft, ⌜κ ∈ invctx_to_multiset Il⌝ -∗ llctx_interp L &&{ ↑NllftG }&&> @[κ])%I as "#Alive". {
       iIntros (κ) "%Hin". destruct Halive as [Halive1 Halive2].
@@ -239,8 +198,7 @@ Section local_invariants.
     iFrame. iFrame "#".
     iDestruct (ty_gho_depth_mono with "gho") as "[$ _]". { lia. } { lia. }
     iSplit. { done. }
-    iApply (proph_obs_impl with "Obs").
-    intros π Ha. apply Ha. trivial.
+    iPureIntro. apply Obs. trivial.
   Qed.
   
   Local Lemma mask_lemma (na_mask at_mask X : coPset) :
@@ -263,11 +221,11 @@ Section local_invariants.
       (Seq Skip Skip)
       (InvCtx (InvCtx_open κ :: Il) ϝ 𝛼)
       (const +[p ◁ own_ptr 0 (tracked_ty ty * local_closer_ty κ ty pred)])
-      (λ post '-[(_, (_, (N, γ, c)))], λ mask π, (↑N ⊆ mask) ∧ ∀ l v γ', pred (syn_abstract v) c → post -[(l, (v, (N, γ', c)))] (mask ∖ ↑N) π).
+      (λ post '-[(_, (_, (N, γ, c)))], λ mask, (↑N ⊆ mask) ∧ ∀ l v γ', pred (syn_abstract v) c → post -[(l, (v, (N, γ', c)))] (mask ∖ ↑N)).
   Proof.
     intros Halive HaliveI. apply typed_inv_instr_of_skip_own_own_t. { trivial. } { trivial. }
     intros l [l1 [[ns [[γ γt] d0]] c]] d tid iκs post mask.
-    iIntros "#LFT #TIME #PROPH #UNIQ #E L I shrgho #Obs #⧖ ⧗ £".
+    iIntros "#LFT #TIME #UNIQ #E L I shrgho %Obs #⧖ ⧗ £".
     iDestruct (lc_weaken (_ + _)%nat with "£") as "[£1 £2]"; first last.
     {
     destruct d as [|d]; first by done.
@@ -283,8 +241,7 @@ Section local_invariants.
     leaf_hyp "KguardsGho" rhs to (cna_active γ) as "KguardsActive".
       { leaf_by_sep. iIntros "(? & ?)". iFrame. iIntros. done. }
     
-    iMod (proph_obs_sat with "PROPH Obs") as "%Sat". { set_solver. }
-    destruct Sat as [π [a b]].
+    destruct Obs as [Sat Obs].
     
     iDestruct "I" as (na_mask at_mask) "[%Hm [[Ilifetimes ϝIncl] [Iown Iat]]]".
     iMod (cna_inv_acc_with_lifetime_guard with "inv Iown Ilifetimes LguardsK £2 KguardsActive L") as "[Iown [Ilifetimes [L [P Closer]]]]". { set_solver. } { set_solver. }
@@ -299,8 +256,7 @@ Section local_invariants.
       { iPureIntro. split; last by set_solver. apply mask_lemma; set_solver. }
       unfold invctx_to_multiset. simpl. rewrite gmultiset_disj_union_assoc. iFrame.
     }
-    iApply (proph_obs_impl with "Obs").
-    intros π0 Ha. apply Ha. trivial.
+    iPureIntro. apply Obs. trivial.
     }
     lia.
   Qed.
@@ -314,14 +270,14 @@ Section local_invariants.
       (Seq Skip Skip)
       (InvCtx Il ϝ 𝛼)
       (const +[])
-      (λ post '-[(_, v); (_, (N, γ, c))], λ mask π,
-        pred (syn_abstract v) c ∧ post -[] (mask ∪ ↑N) π
+      (λ post '-[(_, v); (_, (N, γ, c))], λ mask,
+        pred (syn_abstract v) c ∧ post -[] (mask ∪ ↑N)
       ).
   Proof.
     apply typed_inv_instr_of_skip_own2_emp.
     intros l1 l2 v [[ns [[γ γt] d0]] c] d tid iκs post mask.
-    iIntros "#LFT #TIME #PROPH #UNIQ E L I gho1 [tok closer] #Obs #⧖ ⧗big £d".
-    iMod (proph_obs_sat with "PROPH Obs") as "%Sat". { set_solver. }
+    iIntros "#LFT #TIME #UNIQ E L I gho1 [tok closer] %Obs #⧖ ⧗big £d".
+    destruct Obs as [Sat Obs].
     iDestruct "I" as (na_mask at_mask) "[%Hm [[Ilifetimes ϝIncl] [Iown Iat]]]".
     iMod (cna_close with "closer [gho1 ⧗big £d tok] Iown Ilifetimes") as (κs') "[[%LtsEq %Hdisj] [Iown Ilifetimes]]".
      { solve_ndisj. }
@@ -329,15 +285,14 @@ Section local_invariants.
         iDestruct (persistent_time_receipt_mono with "⧖") as "$"; first lia.
         iDestruct (cumulative_time_receipt_mono with "⧗big") as "$"; first lia.
         iDestruct (lc_weaken with "£d") as "$"; first lia.
-        destruct Sat as [π [a b]]. done.
+        iPureIntro. exact Sat.
      }
     unfold invctx_to_multiset in LtsEq. simpl in LtsEq. 
     assert (invctx_to_multiset Il ⊎ list_to_set_disj iκs = κs') as LtsEq2 by multiset_solver.
     rewrite <- LtsEq2.
     iModIntro. iExists (mask ∪ ↑ns). iFrame.
     iSplit. { iPureIntro. split; set_solver. }
-    iApply (proph_obs_impl with "Obs"). intros π Ha. apply Ha.
+    iPureIntro. exact Obs.
   Qed.
 End local_invariants.
 
-Global Hint Resolve local_inv_ty_resolve : lrust_typing.
