src/lambda_verus/typing/programs_util.v
@@ -6,35 +6,35 @@ From guarding Require Import guard tactics.
 Set Default Proof Using "Type".
 
 Section programs_util.
-  Context `{!typeG Σ}.
+  Context `{!typeG Σ, !cnaInv_logicG Σ}.
   
   Lemma typed_instr_of_skip
     {𝔄 𝔅l} (E: elctx) (L: llctx) (I: invctx)
     (p : path) (ty : type 𝔄)
     (T': tctx 𝔅l) (tr: predl_trans [𝔄] 𝔅l) :
-    (∀ x v d tid post mask iκs, ⊢ (llft_ctx -∗ time_ctx -∗ proph_ctx -∗ uniq_ctx -∗ elctx_interp E -∗
+    (∀ x v d tid post mask iκs, ⊢ (llft_ctx -∗ time_ctx -∗ uniq_ctx -∗ elctx_interp E -∗
       llctx_interp L -∗ invctx_interp tid mask iκs I -∗
       ⌜eval_path p = Some v⌝ -∗ ty_own ty x d d tid [FVal v] -∗
-      ⟨π, tr post -[x] mask π⟩ -∗
+      ⌜tr post -[x] mask⌝ -∗
       ⧖(S d) -∗
       ⧗1 -∗ ⧗1 -∗ £(advance_credits d) -∗ |={⊤}=>
-      ∃ xl' , llctx_interp L ∗ invctx_interp tid mask iκs I ∗ tctx_interp tid T' xl' ∗ ⟨π, post xl' mask π⟩
+      ∃ xl' , llctx_interp L ∗ invctx_interp tid mask iκs I ∗ tctx_interp tid T' xl' ∗ ⌜post xl' mask⌝
     )%I)
     → typed_instr E L I +[p ◁ ty] (Seq Skip Skip) (const T') tr.
   Proof.
     intros Hvs tid post mask iκs xl. destruct xl as [x []].
-    iIntros "#CTX #TIME #PROPH #UNIQ #E L I [T _] Obs".
+    iIntros "#CTX #TIME #UNIQ #E L I [T _] %Obs".
     iDestruct "T" as (v d) "(p & #⧖1 & own)".
     wp_bind Skip.
-    iApply wp_fupd.
-    iApply (wp_persistent_time_receipt with "TIME ⧖1"). { set_solver. } 
+    iApply pgl_wp_fupd.
+    iApply (wp_persistent_time_receipt _ with "TIME ⧖1"); [done|set_solver|]. 
     iIntros "£ #⧖". wp_let. iModIntro. wp_let.
-    iApply wp_fupd.
-    iApply (wp_cumulative_time_receipt2 with "TIME"). { set_solver. } 
+    iApply pgl_wp_fupd.
+    iApply (wp_cumulative_time_receipt2 with "TIME"); [done|set_solver|]. 
     iIntros "⧗". replace 2 with (1 + 1)%nat by done.
     iDestruct (cumulative_time_receipt_sep with "⧗") as "[⧗1 ⧗2]".
     wp_let.
-    iMod (Hvs x v d tid post with "CTX TIME PROPH UNIQ E L I p own Obs ⧖ ⧗1 ⧗2 £") as (xl') "(? & ? & ? & ?)".
+    iMod (Hvs x v d tid post with "CTX TIME UNIQ E L I p own [//] ⧖ ⧗1 ⧗2 £") as (xl') "(? & ? & ? & ?)".
     iModIntro. iFrame.
   Qed.
   
@@ -42,28 +42,28 @@ Section programs_util.
     {𝔄 𝔅l} (E: elctx) (L: llctx) (I: invctx) (I': invctx)
     (p : path) (ty : type 𝔄)
     (T': tctx 𝔅l) (tr: predl_trans [𝔄] 𝔅l) :
-    (∀ x v d tid post mask iκs, ⊢ (llft_ctx -∗ time_ctx -∗ proph_ctx -∗ uniq_ctx -∗ elctx_interp E -∗
+    (∀ x v d tid post mask iκs, ⊢ (llft_ctx -∗ time_ctx -∗ uniq_ctx -∗ elctx_interp E -∗
       llctx_interp L -∗ invctx_interp tid mask iκs I -∗
       ⌜eval_path p = Some v⌝ -∗ ty_own ty x d d tid [FVal v] -∗
-      ⟨π, tr post -[x] mask π⟩ -∗
+      ⌜tr post -[x] mask⌝ -∗
       ⧖(S d) -∗
       ⧗1 -∗ £(advance_credits d) -∗ |={⊤}=>
-      ∃ xl' mask', llctx_interp L ∗ invctx_interp tid mask' iκs I' ∗ tctx_interp tid T' xl' ∗ ⟨π, post xl' mask' π⟩
+      ∃ xl' mask', llctx_interp L ∗ invctx_interp tid mask' iκs I' ∗ tctx_interp tid T' xl' ∗ ⌜post xl' mask'⌝
     )%I)
     → typed_inv_instr E L I +[p ◁ ty] (Seq Skip Skip) I' (const T') tr.
   Proof.
     intros Hvs tid post mask iκs xl. destruct xl as [x []].
-    iIntros "#CTX #TIME #PROPH #UNIQ #E L I [T _] Obs".
+    iIntros "#CTX #TIME #UNIQ #E L I [T _] %Obs".
     iDestruct "T" as (v d) "(p & #⧖1 & own)".
     wp_bind Skip.
-    iApply wp_fupd.
-    iApply (wp_persistent_time_receipt with "TIME ⧖1"). { set_solver. } 
+    iApply pgl_wp_fupd.
+    iApply (wp_persistent_time_receipt _ with "TIME ⧖1"); [done|set_solver|]. 
     iIntros "£ #⧖". wp_let. iModIntro. wp_let.
-    iApply wp_fupd.
-    iApply (wp_cumulative_time_receipt1 with "TIME"). { set_solver. } 
+    iApply pgl_wp_fupd.
+    iApply (wp_cumulative_time_receipt1 with "TIME"); [done|set_solver|]. 
     iIntros "⧗".
     wp_let.
-    iMod (Hvs x v d tid post with "CTX TIME PROPH UNIQ E L I p own Obs ⧖ ⧗ £") as (xl' mask') "(? & ? & ? & ?)".
+    iMod (Hvs x v d tid post with "CTX TIME UNIQ E L I p own [//] ⧖ ⧗ £") as (xl' mask') "(? & ? & ? & ?)".
     iModIntro. iFrame.
   Qed.
    
@@ -72,30 +72,30 @@ Section programs_util.
     (p1 : path) (ty1 : type 𝔄1)
     (p2 : path) (ty2 : type 𝔄2)
     (T': tctx 𝔅l) (tr: predl_trans (𝔄1 :: [𝔄2]) 𝔅l) :
-    (∀ x1 x2 v1 v2 d tid post mask, ⊢ (llft_ctx -∗ time_ctx -∗ proph_ctx -∗ uniq_ctx -∗ elctx_interp E -∗
+    (∀ x1 x2 v1 v2 d tid post mask, ⊢ (llft_ctx -∗ time_ctx -∗ uniq_ctx -∗ elctx_interp E -∗
       llctx_interp L -∗
       ⌜eval_path p1 = Some v1⌝ -∗ ty_own ty1 x1 d d tid [FVal v1] -∗
       ⌜eval_path p2 = Some v2⌝ -∗ ty_own ty2 x2 d d tid [FVal v2] -∗
-      ⟨π, tr post -[x1; x2] mask π⟩ -∗
+      ⌜tr post -[x1; x2] mask⌝ -∗
       ⧖(S d) -∗
       ⧗1 -∗ |={⊤}=>
-      ∃ xl' , llctx_interp L ∗ tctx_interp tid T' xl' ∗ ⟨π, post xl' mask π⟩
+      ∃ xl' , llctx_interp L ∗ tctx_interp tid T' xl' ∗ ⌜post xl' mask⌝
     )%I)
     → typed_instr E L I +[p1 ◁ ty1; p2 ◁ ty2] (Seq Skip Skip) (const T') tr.
   Proof.
     intros Hvs tid post mask iκs xl. destruct xl as [x1 [x2 []]].
-    iIntros "#CTX #TIME #PROPH #UNIQ #E L I [T1 [T2 _]] Obs".
+    iIntros "#CTX #TIME #UNIQ #E L I [T1 [T2 _]] %Obs".
     iDestruct "T1" as (v1 d1) "(p1 & #⧖1 & own1)".
     iDestruct "T2" as (v2 d2) "(p2 & #⧖2 & own2)".
     iCombine "⧖1 ⧖2" as "⧖".
-    wp_bind Skip. iApply wp_fupd.
-    iApply (wp_persistent_time_receipt with "TIME ⧖"). { set_solver. } 
+    wp_bind Skip. iApply pgl_wp_fupd.
+    iApply (wp_persistent_time_receipt _ with "TIME ⧖"); [done|set_solver|]. 
     iIntros "£ #S⧖". wp_let. iModIntro. wp_let.
-    iApply wp_fupd.
-    iApply (wp_cumulative_time_receipt1 with "TIME"). { set_solver. } 
+    iApply pgl_wp_fupd.
+    iApply (wp_cumulative_time_receipt1 with "TIME"); [done|set_solver|]. 
     iIntros "⧗".
     wp_let.
-    iMod (Hvs x1 x2 v1 v2 (d1 `max` d2) tid post with "CTX TIME PROPH UNIQ E L p1 [own1] p2 [own2] Obs S⧖ ⧗") as "J".
+    iMod (Hvs x1 x2 v1 v2 (d1 `max` d2) tid post with "CTX TIME UNIQ E L p1 [own1] p2 [own2] [//] S⧖ ⧗") as "J".
      { iDestruct "own1" as "[gho phys]". iFrame.
        iDestruct (ty_gho_depth_mono with "gho") as "[gho _]"; last by iFrame "gho".
        { lia. } { lia. }
@@ -112,40 +112,41 @@ Section programs_util.
     (p1 : path) (ty1 : type 𝔄1)
     (p2 : path) (ty2 : type 𝔄2)
     (T': tctx 𝔅l) (tr: predl_trans (𝔄1 :: [𝔄2]) 𝔅l) :
-    (∀ x1 x2 v1 v2 d tid post mask iκs, ⊢ (llft_ctx -∗ time_ctx -∗ proph_ctx -∗ uniq_ctx -∗ elctx_interp E -∗
+    (∀ x1 x2 v1 v2 d tid post mask iκs, ⊢ (llft_ctx -∗ time_ctx -∗ uniq_ctx -∗ elctx_interp E -∗
       llctx_interp L -∗ invctx_interp tid mask iκs I -∗
       ⌜eval_path p1 = Some v1⌝ -∗ ty_own ty1 x1 d d tid [FVal v1] -∗
       ⌜eval_path p2 = Some v2⌝ -∗ ty_own ty2 x2 d d tid [FVal v2] -∗
-      ⟨π, tr post -[x1; x2] mask π⟩ -∗
+      ⌜tr post -[x1; x2] mask⌝ -∗
       ⧖(S d) -∗
       ⧗d -∗
       ⧗1 -∗
       £d -∗
       |={⊤}=>
-      ∃ xl' mask' , llctx_interp L ∗ invctx_interp tid mask' iκs I' ∗ tctx_interp tid T' xl' ∗ ⟨π, post xl' mask' π⟩
+      ∃ xl' mask' , llctx_interp L ∗ invctx_interp tid mask' iκs I' ∗ tctx_interp tid T' xl' ∗ ⌜post xl' mask'⌝
     )%I)
     → typed_inv_instr E L I +[p1 ◁ ty1; p2 ◁ ty2] (Seq Skip Skip) I' (const T') tr.
   Proof.
     intros Hvs tid post mask iκs xl. destruct xl as [x1 [x2 []]].
-    iIntros "#CTX #TIME #PROPH #UNIQ #E L I [T1 [T2 _]] Obs".
+    iIntros "#CTX #TIME #UNIQ #E L I [T1 [T2 _]] %Obs".
     iDestruct "T1" as (v1 d1) "(p1 & #⧖1 & own1)".
     iDestruct "T2" as (v2 d2) "(p2 & #⧖2 & own2)".
     iCombine "⧖1 ⧖2" as "⧖".
-    wp_bind Skip. iApply wp_fupd.
-    iApply (wp_cumulative_time_receipt2 with "TIME"). { set_solver. } 
+    wp_bind Skip. iApply pgl_wp_fupd.
+    iApply (wp_cumulative_time_receipt2 with "TIME"); [done|set_solver|]. 
     iIntros "⧗". wp_let. iModIntro. wp_let.
     replace 2 with (1 + 1)%nat by done.
     iDestruct (cumulative_time_receipt_sep with "⧗") as "[⧗1 ⧗2]".
+    iApply fupd_pgl_wp.
     iMod (cumulative_persistent_time_receipt_get_credits with "TIME ⧗1 ⧖") as "[#S⧖ £]"; first by set_solver.
     iDestruct (lc_weaken with "£") as "£"; last first. {
-    iApply wp_fupd.
+    iApply pgl_wp_fupd.
     replace (d1 `max` d2 + 1) with (S (d1 `max` d2)) by lia.
-    iApply (wp_cumulative_time_receipt_linear with "TIME S⧖"). { set_solver. } 
-    iIntros "⧗big".
+    iApply (wp_cumulative_time_receipt_linear _ _ _ (S (d1 `max` d2)) with "TIME S⧖"); [done|set_solver|].
+    iModIntro. iIntros "⧗big".
     wp_let.
     replace (S (S (S (d1 `max` d2)))) with (d1 `max` d2 + 3)%nat by lia.
     iDestruct "⧗big" as "[⧗big ⧗3]".
-    iMod (Hvs x1 x2 v1 v2 (d1 `max` d2) tid post with "CTX TIME PROPH UNIQ E L I p1 [own1] p2 [own2] Obs S⧖ ⧗big ⧗2 £") as "J".
+    iMod (Hvs x1 x2 v1 v2 (d1 `max` d2) tid post with "CTX TIME UNIQ E L I p1 [own1] p2 [own2] [//] S⧖ ⧗big ⧗2 £") as "J".
      { iDestruct "own1" as "[gho phys]". iFrame.
        iDestruct (ty_gho_depth_mono with "gho") as "[gho _]"; last by iFrame "gho".
        { lia. } { lia. }
@@ -164,35 +165,37 @@ Section programs_util.
     (ty : type 𝔄)
     (ty' : type 𝔅)
     (tr: predl_trans' [𝔄] 𝔅) :
-    (∀ x v d tid post mask, ⊢ (llft_ctx -∗ time_ctx -∗ proph_ctx -∗ uniq_ctx -∗ elctx_interp E -∗
+    (∀ x v d tid post mask, ⊢ (llft_ctx -∗ time_ctx -∗ uniq_ctx -∗ elctx_interp E -∗
       llctx_interp L -∗
       ⌜eval_path p = Some v⌝ -∗ ty_own ty x d d tid [FVal v] -∗
-      ⟨π, tr post -[x] mask π⟩ -∗
+      ⌜tr post -[x] mask⌝ -∗
       ⧗1 -∗
       ⧖(d) -∗
       £(2*d*d + 4*d + 2) -∗ |={⊤ ∖ ↑advN}=> ∃ (l: cloc) (l': loc) H, ⌜v = #l.1⌝ ∗ H ∗ (H &&{↑NllftG; d+1}&&> (l.1 ↦[^ l.2]∗ [ #l' ])) ∗ (H ={⊤}=∗
-      ∃ x' , llctx_interp L ∗ ty_own ty' x' d d tid [FVal #l' ] ∗ ⟨π, post x' mask π⟩
+      ∃ x' , llctx_interp L ∗ ty_own ty' x' d d tid [FVal #l' ] ∗ ⌜post x' mask⌝
     ))%I)
     → typed_instr_ty E L I +[p ◁ ty] (!p) (ty') tr.
   Proof. 
     intros Rd tid post mask iκs xl. destruct xl as [x []].
-    iIntros "#LFT #TIME #PROPH #UNIQ #E L I [T _] Obs".
+    iIntros "#LFT #TIME #UNIQ #E L I [T _] %Obs".
     wp_bind p.
     iApply (wp_hasty with "T").
     iIntros (v d) "%Hp #⧖ ty".
-    iApply wp_fupd.
-    iApply (wp_cumulative_time_receipt2 with "TIME"); first by set_solver.
+    iApply pgl_wp_fupd.
+    iApply (wp_cumulative_time_receipt2 with "TIME"); [done|set_solver|].
     iIntros "⧗". replace 2 with (1 + 1); last by done.
     iDestruct (cumulative_time_receipt_sep with "⧗") as "[⧗1 ⧗2]".
+    iApply fupd_pgl_wp.
     iMod (cumulative_persistent_time_receipt_get_credits with "TIME ⧗1 ⧖") as "[⧖' £]";
         first by solve_ndisj.
     iDestruct (lc_weaken (_ + _)%nat with "£") as "[£1 £2]"; first last. {
-    iMod (Rd x v d tid with "LFT TIME PROPH UNIQ E L [] ty Obs ⧗2 ⧖ £1") as (l l' H) "[%Hvl [H [#Hpt VsBack]]]"; first by trivial.
+    iMod (Rd x v d tid with "LFT TIME UNIQ E L [] ty [//] ⧗2 ⧖ £1") as (l l' H) "[%Hvl [H [#Hpt VsBack]]]"; first by trivial.
     subst v.
-    iApply (wp_read_na_guarded_cells_singleton with "[H £2]"); first by solve_ndisj.
+    iApply (wp_read_guarded_singleton with "[H £2]"); first by solve_ndisj.
      { iFrame "Hpt". iFrame "H". iFrame "£2". }
-    iNext. iIntros "H". iMod ("VsBack" with "H") as (x') "(L & Ty' & #Obs)".
-    iModIntro. iExists -[x']. iFrame. iFrame "#". done.
+    iIntros "!> !> H". iMod ("VsBack" with "H") as (x') "(L & Ty' & %Obs')".
+    iModIntro. iExists -[x']. iFrame.
+    iSplit; last by iPureIntro. iSplit; [done|iFrame "⧖"].
     }
     unfold advance_credits. lia.
   Qed.
@@ -203,34 +206,36 @@ Section programs_util.
     (ty : type 𝔄)
     (ty' : type 𝔅)
     (tr: predl_trans' [𝔄] (𝔅)) :
-    (∀ x v d tid post mask, ⊢ (llft_ctx -∗ time_ctx -∗ proph_ctx -∗ uniq_ctx -∗ elctx_interp E -∗
+    (∀ x v d tid post mask, ⊢ (llft_ctx -∗ time_ctx -∗ uniq_ctx -∗ elctx_interp E -∗
       llctx_interp L -∗
       ⌜eval_path p = Some v⌝ -∗ ty_own ty x d d tid [FVal v] -∗
-      ⟨π, tr post -[x] mask π⟩ -∗
+      ⌜tr post -[x] mask⌝ -∗
       ⧖(d) -∗
       £(2*d*d + 4*d + 2) -∗ |={⊤ ∖ ↑advN}=> ∃ (l: cloc) (l': loc) H, ⌜v = #l.1⌝ ∗ H ∗ (H &&{↑NllftG; d+1}&&> (l.1 ↦[^ l.2]∗ [ #l' ])) ∗ (H ={⊤}=∗
-      ∃ x' , llctx_interp L ∗ ty_own ty' x' (S d) (S d) tid [FVal #l' ] ∗ ⟨π, post x' mask π⟩
+      ∃ x' , llctx_interp L ∗ ty_own ty' x' (S d) (S d) tid [FVal #l' ] ∗ ⌜post x' mask⌝
     ))%I)
     → typed_instr_ty E L I +[p ◁ ty] (!p) (ty') tr.
   Proof.
     intros Rd tid post mask iκs xl. destruct xl as [x []].
-    iIntros "#LFT #TIME #PROPH #UNIQ #E L I [T _] Obs".
+    iIntros "#LFT #TIME #UNIQ #E L I [T _] %Obs".
     
     wp_bind p.
     iApply (wp_hasty with "T").
     iIntros (v d) "%Hp #time ty".
-    iApply (wp_fupd).
-    iApply (wp_persistent_time_receipt with "TIME time"). { set_solver. }
+    iApply pgl_wp_fupd.
+    iApply (wp_persistent_time_receipt _ with "TIME time"); [done|set_solver|].
     iIntros "H£ #⧖S".
     iDestruct (lc_weaken (_ + _)%nat with "H£") as "[£1 £2]"; first last.
     {
-    iApply fupd_wp; iMod (fupd_mask_subseteq (⊤∖↑advN)). { trivial. }
-    iMod (Rd x v d tid with "LFT TIME PROPH UNIQ E L [] ty Obs time £1") as (l l' H) "[%Hvl [H [#Hpt VsBack]]]"; first by trivial.
+    iApply fupd_pgl_wp; iMod (fupd_mask_subseteq (⊤∖↑advN)) as "Hcl". { trivial. }
+    iMod (Rd x v d tid with "LFT TIME UNIQ E L [] ty [//] time £1") as (l l' H) "[%Hvl [H [#Hpt VsBack]]]"; first by trivial.
     subst v.
     
-    iApply (wp_read_na_guarded_cells_singleton with "[H £2]"). { solve_ndisj. } { iFrame "Hpt". iFrame "H". iFrame "£2". }
-    iModIntro. iNext. iIntros "H". iMod ("VsBack" with "H") as (x') "(L & Ty' & #Obs)".
-    iModIntro. iExists -[x']. iFrame. iFrame "#". done.
+    iMod "Hcl" as "_".
+    iApply (wp_read_guarded_singleton with "[H £2]"). { solve_ndisj. } { iFrame "Hpt". iFrame "H". iFrame "£2". }
+    iIntros "!> !> H". iMod ("VsBack" with "H") as (x') "(L & Ty' & %Obs')".
+    iModIntro. iExists -[x']. iFrame.
+    iSplit; last by iPureIntro. iSplit; [done|iFrame "⧖S"].
     } unfold advance_credits; lia.
   Qed.
   
